src/Coq/env.v
@@ -1,0 +1,138 @@
+Require Import Metatheory.
+Import List.
+Import ListNotations.
+(*
+Definition env (A:Type) := list (id * A).
+
+Fixpoint get {A: Type} (m: env A) (x: id): option A :=
+  match m with
+  | nil => None
+  | (x1, a) :: ms =>
+    if (beq_id x x1) then Some a
+    else get ms x
+  end.
+Locate "*".
+SearchAbout prod.
+ Only update our env if x is not defined yet
+   This will ensure a well formed env *)
+Inductive env {A: Type}: list (id * A) -> Type :=
+  | env_nil : env nil
+(*  | ext_single : forall x a,
+    env [(x, a)]*)
+  | env_ext : forall e x b,
+    env e ->
+    ~In x (map fst e)->
+    env ((x,b):: e).
+Hint Constructors env.
+(*
+Inductive get {A: Type} : env A -> id -> Prop:=
+  | get_head : forall x b e, get ((x,b)::e) b
+  .
+*)
+
+Fixpoint get {A: Type} {l: list (id * A)} (m: env l) (x: id): option A :=
+  match m  with
+  | env_nil => None
+  | env_ext _ x1 a en _ =>
+    if (beq_id x x1) then Some a
+    else get en x
+  end.
+Notation " m 'extds' ids ':' vals" := (env (m ++ combine ids vals)) (at level 20, ids at next level).
+
+Lemma get_if_in : forall (A: Type) (l: list (id * A)) (e: env l) x (Bi:A) e,
+  @get A l e x = Some Bi ->
+  In x (map fst l).
+Proof.
+  intros.
+  induction e.
+  simpl.
+  unfold get in H.
+  case e0.
+  inversion H.
+  rewrite e0 in H.
+  inversion H.
+
+Lemma exists_bs : forall (A: Type) Gamma xs (Bs: list A) (e: Gamma extds xs : Bs) x Bi,
+  get e x = Some Bi ->
+  exists i, nth_error Bs i = Some Bi.
+Proof.
+  intros.
+  induction env0. inversion H.
+  apply IHenv0. inversion H.
+  assert (In x (map fst e)).
+ subst.
+
+Lemma env_1 : env [(Id 1, 100); (Id 2, 200); (Id 3, 300)].
+Proof.
+  repeat constructor; eauto.
+  simpl. intro. inversion H. inversion H0. auto.
+  simpl.
+  intro.
+  destruct H; auto. inversion H.
+  destruct H; inversion H.
+Qed.
+
+
+Eval compute in (get env_1 (Id 1)).
+
+Lemma env_
+
+Lemma get_ex : get env_1 (Id 1) = Some 100.
+Proof.
+  unfold get.
+  simpl.
+
+Definition extend {A: Type} (m: env A) (x: id) (a: A) :=
+  match (get m x) with
+  | None => (x, a) :: m
+  | _ => m
+  end.
+Notation " m 'extd' id ':' val" := (extend m id val) (at level 20, id at next level).
+
+Inductive is_in_env {A: Type} (m: env A) (x: id) : Prop:=
+  | is_in : forall a, get m x = Some a -> is_in_env m x.
+Notation "x 'is_in' m" := (is_in_env m x) (at level 40). 
+
+Fixpoint extend_list {B: Type} (m: env B) (xs: list id) (bs: list B): (env B) :=
+  match xs, bs with
+  | x :: xs', b :: bs' => extend_list (extend m x b) xs' bs'
+  | _ , _ => m
+  end.
+Notation " m 'extds' ids ':' vals" := (extend_list m ids vals) (at level 20, ids at next level).
+
+Inductive wf_env {A: Type} (m: env A) : Prop:=
+  | wf1 : wf_env []
+  | wf2 : forall, 
+
+Lemma update_not_shadow: forall {A: Type} (m: env A) x a,
+  x is_in m ->
+  (m extd x : a) = m.
+Proof.
+  intros; case m in *. inversion H. inversion H0.
+  inversion H.
+  unfold extend.
+  rewrite H0. auto.
+Qed.
+
+Theorem extend_neq : forall (X:Type) v x1 x2 (m : env X),
+x2 <> x1 -> 
+get (extend m x2 v) x1 = get m x1.
+Proof.
+intros X v x1 x2 m H.
+unfold extend.
+case (get m x2); auto. simpl.
+rewrite not_eq_beq_id_false; auto.
+Qed.
+
+Lemma extend_list_not_shadow: forall A (m: env A) x xs bs,
+  ~In x xs ->
+  get (m extds xs : bs) x = get m x.
+Proof.
+  intros; gen xs bs.
+  induction xs, bs; auto.
+  apply not_in_cons in H. destruct H.
+  simpl.
+  unfold extend.
+  destruct (get m a) eqn:Heq. apply IHxs; auto.
+Admitted.
+  
